

# • Graph

1. Graph Isomorphism 图同构  $1, 1, 2, 4, 11, 34 \dots$

2. Euler Theorem ① 欧拉回路 节点度数为偶数且连通

② 欧拉路径 0/2个奇度数节点、连通 [两奇节点路径+欧拉回路]

3. matching a set  $M \subseteq E$  s.t. no edges share an endpoint

① perfect matching 点覆盖

② maximum matching 最多

③ bipartite matching [2-colorable / 无奇环]

$\begin{cases} K_n & n \text{ 点完全图} \\ K_{m,n} & \text{二分图 } |V_1|=m, |V_2|=n \end{cases}$

Hall Theorem: bipartite graph  $G=(V, W, E)$  has a perfect matching iff  $|N(S)| \geq |S|$

for each subset  $S$  of  $V$  and  $W$ .  $[N(S) = \{v \mid v \text{ is a neighbor of some vertex in } S\}]$

\* if  $S \subseteq X$   $|N(S)| < |S|$ , then  $S$  与  $N(S)$  不相交

if  $\exists v_0 \in N(S) \mid v_0 \text{ matches with } v_0 \in X \setminus S$ , then  $|S|$  need to match with  $|N(S)|-1$  vertex, which is an impossible case (Actually,  $S$  only equals  $\emptyset$  or  $X$ )

## ④ stable matching

[unstable:  $(b, g) \notin M$  but both prefer each other over their current partners in  $M$ ]

Gale-Shapley Theorem: 1° free boys propose to best no-yet-proposed girl

2° each girl keeps her favorite proposal (tentative) and reject others

3° rejected boys try next turn

4° within  $n^2$  turns to be a stable match

4. coloring ①  $\chi(G) \geq \omega(G)$   $\omega(G)$  为最大完全子图

②  $\chi(G) \leq k+1$  maximum  $\deg(V) = k$

③ interval graph  $\chi(G) = \omega(G)$   $\chi(G) \leq \omega(G)$  按左端点排序, 当染某一节点时, 其相邻节点中左端点小于该点的  $\leq \omega(G)-1 \Rightarrow \chi(G) = \omega(G)$

④ Euler's formula  $V - E + F = 2$   $k$ -connected  $V - E + F = k + 1$

⑤ Planar graph 1°  $\sum_{f \in F} \deg(f) = 2E$  平面图即可

2°  $\sum \deg(f) \geq 3F$  简单平面图

推论:

1°  $2E \geq 3F, V - E + F = 2 \Rightarrow F \leq 3V - 6$  (简单平面图)

2° 存在度数  $\leq 5$  的点  $v_0$   $[2E = \sum \deg(v) \geq 6V \Rightarrow E \geq 3V \text{ contradicts with } E \leq 3V - 6]$   $[K_5]$

3° 无三角形存在时  $2E = \sum \deg(f) \geq 4F \Rightarrow F \leq \frac{E}{2} \Rightarrow E \leq 2V - 4$   $[K_{3,3}]$

4° 6-coloring 由2°可知将  $v_0$  删除后染色,  $v_0$  必能染色, 重复即可.



• gcd & fibonacci:

1.  $\gcd(a,b) \mid \gcd(a,bc)$

$$\begin{cases} \gcd(a,b) \mid b \Rightarrow \gcd(a,b) \mid bc \\ \gcd(a,b) \mid a \end{cases} \Rightarrow \gcd(a,b) \mid \gcd(a,bc)$$

2.  $b \mid a \Leftrightarrow \gcd(a,b) = b$

① if  $a = kb$   $\gcd(a,b) = \gcd(b, a \% b) = b$

② Assume  $b \nmid a$ . let  $a = kb + r$  ( $0 < r < b$ )

$$\gcd(a,b) = \gcd(b,r) < b \text{ contradiction!} \Rightarrow b \mid a$$

3. if  $\gcd(a,c) = 1$ , then  $\gcd(a,bc) = \gcd(a,b)$

① by 1 we know  $\gcd(a,b) \leq \gcd(a,bc) \Rightarrow \gcd(a,bc) = \gcd(a,b)$

②  $\gcd(ab,bc) = \gcd(a,c) \times b = b \geq \gcd(a,b)$

4. if  $b \mid c$ , then  $\gcd(a,b) = \gcd(a+c,b)$

$$\gcd(a+c,b) = \gcd(a \% b, b) = \gcd(a,b)$$

5.  $\gcd(f_n, f_{n-1}) = 1$  [  $f_n$  fibonacci sequence:  $\overset{f_0}{\downarrow} 0, 1, 1, 2, 3 \dots$  ]

$$\gcd(f_n, f_{n-1}) = \gcd(f_{n-1}, f_n - f_{n-1}) = \gcd(f_{n-1}, f_{n-2}) = \dots = \gcd(f_1, f_0) = 1$$

6.  $f_{n+m} = f_{n-1} f_m + f_n f_{m+1}$

method 1: prove by induction

①  $m=1$ ,  $f_{n+1} = f_{n-1} \cdot 1 + f_n \cdot 1$

②  $m=2$ ,  $f_{n+2} = f_{n-1} + f_3 f_n = f_n + (f_n + f_{n-1}) = f_{n+1} + f_n$

③  $P(m), P(m+1) \Rightarrow P(m+r)$

$$f_{n+m+2} = f_{n+m+1} + f_{n+m} = f_{n-1} (f_m + f_{m+1}) + f_n (f_{m+2} + f_{m+1}) = f_{n-1} \cdot f_{m+2} + f_n \cdot f_{m+3}$$

method 2:

if  $m \mid n$ , then  $f_m \mid f_n$

$$\begin{bmatrix} f_{n+2} & f_{n+1} \\ f_{n+1} & f_n \end{bmatrix} = \begin{bmatrix} 1 & 1 \\ 1 & 0 \end{bmatrix}^{n+1}$$

$$f_{n+m} = \left( \begin{bmatrix} 1 & 1 \\ 1 & 0 \end{bmatrix}^{n+m-1} \right)_{1,1} = \left( \begin{bmatrix} 1 & 1 \\ 1 & 0 \end{bmatrix}^n \begin{bmatrix} 1 & 1 \\ 1 & 0 \end{bmatrix}^{m-1} \right)_{1,1} = \left( \begin{bmatrix} f_{n+1} & f_n \\ f_n & f_{n-1} \end{bmatrix} \begin{bmatrix} f_m & f_{m-1} \\ f_{m-1} & f_{m-2} \end{bmatrix} \right)_{1,1} = f_{n-1} f_m + f_n f_{m+1}$$

7.  $\gcd(f_n, f_m) = f_{\gcd(n,m)}$  let  $m < n$

$$\gcd(f_n, f_{n+m}) = \gcd(f_n, f_{n-1} f_m + f_n f_{m+1})$$

$$= \gcd(f_n, f_{n-1} f_m) \quad [\text{since } \gcd(f_n, f_{n-1}) = 1]$$

$$= \gcd(f_n, f_m)$$

$$\Rightarrow \gcd(f_n, f_{n+m}) = \gcd(f_n, f_m) = \dots = \gcd(f_{\gcd(n,m)}, f_0) = f_{\gcd(n,m)}$$

$$8. \gcd(a^k, b^k) = \gcd^k(a, b)$$

$$\gcd(a^k, b^k) = \gcd^k(a, b) \left[ \gcd\left(\left[\frac{a}{\gcd(a, b)}\right]^k, \left[\frac{b}{\gcd(a, b)}\right]^k\right) \right] = \gcd^k(a, b)$$